Fix polynomial.

code/c/Yazi_CRC32Table_Codegen.c
@@ -1,0 +1,16 @@
+#include <stdio.h>
+#include <stdint.h>
+#include "Yazi_CRC32Table.h"
+
+int main(int argc, const char **argv) {
+  uint32_t table[4][256];
+  gen_crc32_table(table[0], table[1], table[2], table[3]);
+
+  for (int i = 0; i < 1; i++) {
+    for (int j = 0; j < 256; j++) { 
+      printf("0x%.8x ", table[i][j]);
+    }
+  }
+  
+  return 0;
+}
